src/program_proof/simplepb/apps/kv_vsm_proof.v
@@ -1,0 +1,772 @@
+From Perennial.program_proof Require Import grove_prelude.
+From Goose.github_com.mit_pdos.gokv.simplepb.apps Require Import kv.
+From Perennial.program_proof Require Import marshal_stateless_proof.
+From iris.base_logic Require Import ghost_map.
+From iris.algebra Require Import mono_list.
+From Perennial.program_proof.simplepb.simplelog Require Import proof.
+From Perennial.program_proof.simplepb Require Import pb_definitions.
+From Perennial.program_proof Require Import map_string_marshal_proof.
+From Perennial.program_proof.aof Require Import proof.
+From Perennial.program_proof.simplepb Require Import config_proof.
+From Perennial.program_proof.simplepb.apps Require Import vsm log.
+From Perennial.program_proof.fencing Require Import map.
+
+Section global_proof.
+
+Inductive kvOp :=
+  | putOp : string → string → kvOp
+  | getOp : string → kvOp
+.
+
+Definition apply_op (state:gmap string string) (op:kvOp) :=
+  match op with
+    | getOp _ => state
+    | putOp k v => <[k:=v]> state
+  end
+.
+
+Definition compute_state ops : gmap string string :=
+  foldl apply_op ∅ ops.
+
+Definition compute_reply ops op : list u8 :=
+  match op with
+    | getOp k => string_to_bytes (default "" ((compute_state ops) !! k))
+    | putOp k v => []
+  end
+.
+
+Definition encode_op op : list u8 :=
+  match op with
+    | putOp k v => [U8 0] ++ u64_le (length (string_to_bytes k)) ++
+                         string_to_bytes k ++ string_to_bytes v
+    | getOp k => [U8 1] ++ string_to_bytes k
+  end
+.
+
+Definition is_readonly_op (op:kvOp) :=
+  match op with
+    | getOp _ => True
+    | _ => False
+  end
+.
+
+Instance op_eqdec : EqDecision kvOp.
+Proof. solve_decision. Qed.
+
+Definition kv_record : Sm.t :=
+  {|
+    Sm.OpType := kvOp ;
+    Sm.has_op_encoding := λ op_bytes op, encode_op op = op_bytes ;
+    Sm.has_snap_encoding := λ snap_bytes ops, has_string_map_encoding snap_bytes (compute_state ops) ;
+    Sm.compute_reply :=  compute_reply ;
+    Sm.is_readonly_op :=  is_readonly_op ;
+    Sm.apply_postcond :=  λ ops op, True ;
+  |}.
+
+Notation OpType := (Sm.OpType kv_record).
+Notation has_op_encoding := (Sm.has_op_encoding kv_record).
+(* Notation compute_reply := (pb_compute_reply pb_record). *)
+Notation pbG := (pbG (pb_record:=kv_record)).
+Notation is_ApplyFn := (is_ApplyFn (pb_record:=kv_record)).
+Notation is_pb_host := (is_pb_host (pb_record:=kv_record)).
+
+Class kvG Σ := KvG {
+  kv_ghostMapG :> ghost_mapG Σ string string ;
+  kv_logG :> inG Σ (mono_listR (leibnizO kvOp)) ;
+  kv_vsmG :> vsmG (sm_record:=kv_record) Σ ;
+}.
+Definition kvΣ := #[configΣ; ghost_mapΣ string string;
+                      GFunctor (mono_listR (leibnizO kvOp));
+                      vsmΣ (sm_record:=kv_record)
+   ].
+Global Instance subG_kvΣ {Σ} : subG kvΣ Σ → kvG Σ.
+Proof. intros. solve_inG. Qed.
+
+Context `{!gooseGlobalGS Σ}.
+Context `{!kvG Σ}.
+
+(* The abstract state applies the operation to an all-nil map,
+   so that each key already exists from the start. This is consisent with
+   [getOp] doing [default []]. *)
+Definition own_kvs (γkv:gname) ops : iProp Σ :=
+  ∃ allocatedKeys,
+  ghost_map_auth γkv 1 (compute_state ops ∪ gset_to_gmap "" allocatedKeys)
+.
+
+Definition stateN := nroot .@ "state".
+
+Definition kv_inv γlog γkv : iProp Σ :=
+  inv stateN ( ∃ ops, own_log γlog ops ∗ own_kvs γkv ops).
+
+Definition kv_ptsto γkv (k v : string) : iProp Σ :=
+  k ↪[γkv] v.
+
+Lemma alloc_kv γlog allocated :
+  own_log γlog [] ={⊤}=∗
+  ∃ γkv ,
+  kv_inv γlog γkv ∗
+  [∗ set] k ∈ allocated, kv_ptsto γkv k ""
+.
+Proof.
+  iIntros "Hlog".
+  iMod (ghost_map_alloc (gset_to_gmap "" allocated)) as (γkv) "[Hkvs Hkvptsto]".
+  iExists _.
+  iMod (inv_alloc with "[Hkvs Hlog]") as "$".
+  { iNext. iExists _; iFrame. rewrite /own_kvs /compute_state /=.
+    iExists _. rewrite left_id_L. done. }
+  replace allocated with (dom (gset_to_gmap "" allocated)) at 2.
+  2:{ rewrite dom_gset_to_gmap. done. }
+  iApply big_sepM_dom. iApply (big_sepM_impl with "Hkvptsto").
+  iIntros "!# %k %x".
+  rewrite lookup_gset_to_gmap_Some.
+  iIntros ([_ <-]). auto.
+Qed.
+
+End global_proof.
+
+Section local_proof.
+
+Notation OpType := (Sm.OpType kv_record).
+Notation has_op_encoding := (Sm.has_op_encoding kv_record).
+(* Notation compute_reply := (pb_compute_reply pb_record). *)
+Notation pbG := (pbG (pb_record:=kv_record)).
+Notation is_ApplyFn := (is_ApplyFn (pb_record:=kv_record)).
+Notation is_pb_host := (is_pb_host (pb_record:=kv_record)).
+
+Context `{!heapGS Σ}.
+Context `{!kvG Σ}.
+
+Lemma wp_encodePutArgs (args_ptr:loc) (key val:string) :
+  {{{
+      "Hargs_key" ∷ args_ptr ↦[kv.PutArgs :: "Key"] #(str key) ∗
+      "Hargs_val" ∷ args_ptr ↦[kv.PutArgs :: "Val"] #(str val)
+  }}}
+    kv.encodePutArgs #args_ptr
+  {{{
+        enc enc_sl, RET (slice_val enc_sl);
+        ⌜ has_op_encoding enc (putOp key val)⌝ ∗
+        own_slice enc_sl byteT 1 enc
+  }}}.
+Proof.
+  iIntros (Φ) "H1 HΦ".
+  iNamed "H1".
+  wp_call.
+  wp_apply (wp_NewSliceWithCap (V:=u8)).
+  { done. }
+  iIntros (ptr) "Hbuf".
+  wp_apply wp_ref_to; first by val_ty. iIntros (l) "Hl".
+  wp_load.
+  iDestruct (own_slice_small_acc with "Hbuf") as "[Hbuf Hbufclose]".
+  wp_apply (wp_SliceSet with "[$Hbuf]").
+  { iPureIntro. done. }
+  iEval simpl.
+  change (<[int.nat 0%Z:=U8 0]> (replicate (int.nat 1%Z) (U8 0))) with [U8 0].
+  iIntros "Hbuf". iDestruct ("Hbufclose" with "Hbuf") as "Hbuf".
+  wp_loadField. wp_load.
+  wp_apply (wp_WriteInt with "Hbuf"). iIntros (sl) "Hbuf". wp_store. clear ptr.
+  wp_loadField.
+  wp_apply wp_StringToBytes.
+  iIntros (?) "Hsl".
+  wp_load.
+  iDestruct (own_slice_to_small with "Hsl") as "Hsl".
+  wp_apply (wp_WriteBytes with "[$Hbuf $Hsl]").
+  iIntros (sl') "[Hbuf _]".
+  wp_store. clear sl.
+  wp_loadField.
+  wp_apply wp_StringToBytes.
+  iIntros (?) "Hsl".
+  wp_load.
+  iDestruct (own_slice_to_small with "Hsl") as "Hsl".
+  wp_apply (wp_WriteBytes with "[$Hbuf $Hsl]").
+  iIntros (?) "[Hbuf _]".
+  wp_store. clear sl.
+  wp_load.
+  iApply "HΦ". iModIntro. iFrame.
+  iPureIntro.
+  by rewrite string_bytes_length.
+Qed.
+
+Lemma wp_decodePutArgs enc_sl enc q (key val:string) :
+  {{{
+        "%Henc" ∷ ⌜has_op_encoding enc (putOp key val)⌝ ∗
+        "Hsl" ∷ own_slice_small enc_sl byteT q enc
+  }}}
+    kv.decodePutArgs (slice_val enc_sl)
+  {{{
+        (args_ptr:loc), RET #args_ptr;
+        "Hargs_key" ∷ args_ptr ↦[kv.PutArgs :: "Key"] #(str key) ∗
+        "Hargs_val" ∷ args_ptr ↦[kv.PutArgs :: "Val"] #(str val)
+  }}}.
+Proof.
+  iIntros (Φ) "Hpre HΦ". iNamed "Hpre".
+  wp_call.
+
+  (* IDEA: maybe get rid of redundancy in slice length by having the slice object be
+     (own_slice_small byteT slptr cap l)
+     (slice_val sl_ptr lst).
+     So instead of an arbitrary `enc_sl`, we should really have `Slice.mk
+     enc_ptr (length enc) enc_cap`, but written more compactly.
+   *)
+  iDestruct (own_slice_small_sz with "Hsl") as %Hsl_sz.
+  cbn in Henc.
+  subst.
+  wp_apply wp_SliceSkip.
+  { cbn in Hsl_sz. word. }
+  iDestruct (slice_small_split _ 1 with "Hsl") as "[_ Hsl]".
+  { cbn. word. }
+  rewrite skipn_cons drop_0.
+  wp_apply (wp_ref_to).
+  { done. }
+  iIntros (enc_ptr) "Henc".
+  wp_pures.
+  wp_apply (wp_allocStruct).
+  { Transparent slice.T. repeat econstructor. Opaque slice.T. }
+  iIntros (args_ptr) "Hargs".
+  iDestruct (struct_fields_split with "Hargs") as "HH".
+  iNamed "HH".
+  wp_pures.
+  wp_apply wp_ref_of_zero.
+  { done. }
+  iIntros (?) "Hl".
+  wp_load.
+  wp_apply (wp_ReadInt with "[$Hsl]").
+  iIntros (kv_sl) "Hkv_sl".
+  wp_pures. wp_store. wp_store. wp_load. wp_load.
+  iDestruct (own_slice_small_wf with "Hkv_sl") as %Hkv_wf.
+  iDestruct (own_slice_small_sz with "Hkv_sl") as %Hkv_sz.
+  simpl in Hsl_sz. rewrite app_length in Hkv_sz.
+  wp_apply wp_SliceTake.
+  { word. }
+  iDestruct (slice_small_split with "Hkv_sl") as "[Hk Hv]".
+  { shelve. }
+  replace (int.nat (length (string_to_bytes key))) with (length (string_to_bytes key)) by word.
+  Unshelve.
+  2:{ rewrite app_length. word. }
+  wp_apply (wp_StringFromBytes with "[$Hk]").
+  iIntros "Hk".
+  rewrite take_app.
+  wp_storeField.
+  rewrite drop_app.
+  wp_load.
+  wp_load.
+  wp_apply wp_SliceSkip.
+  { word. }
+  wp_apply (wp_StringFromBytes with "[$Hv]").
+  iIntros "Hv".
+  do 2 rewrite string_to_bytes_inj.
+  wp_storeField.
+  iModIntro. iApply "HΦ".
+  iFrame.
+Qed.
+
+Lemma wp_encodeGetArgs (key:string) :
+  {{{
+        True
+  }}}
+    kv.encodeGetArgs #(str key)
+  {{{
+        enc enc_sl, RET (slice_val enc_sl);
+        ⌜has_op_encoding enc (getOp key)⌝ ∗
+        own_slice enc_sl byteT 1 enc
+  }}}.
+Proof.
+  iIntros (Φ) "H1 HΦ".
+  iNamed "H1".
+  wp_call.
+  wp_apply (wp_NewSliceWithCap (V:=u8)).
+  { done. }
+  iIntros (ptr) "Hbuf".
+  wp_apply wp_ref_to; first by val_ty. iIntros (l) "Hl".
+  wp_load.
+  iDestruct (own_slice_small_acc with "Hbuf") as "[Hbuf Hbufclose]".
+  wp_apply (wp_SliceSet with "[$Hbuf]").
+  { iPureIntro. done. }
+  iEval simpl.
+  change (<[int.nat 0%Z:=U8 1]> (replicate (int.nat 1%Z) (U8 0))) with [U8 1].
+  iIntros "Hbuf". iDestruct ("Hbufclose" with "Hbuf") as "Hbuf".
+  wp_apply wp_StringToBytes.
+  iIntros (?) "Hsl".
+  wp_load.
+  iDestruct (own_slice_to_small with "Hsl") as "Hsl".
+  wp_apply (wp_WriteBytes with "[$Hbuf $Hsl]").
+  iIntros (?) "[Hbuf _]". wp_store. clear ptr.
+  wp_load.
+  iApply "HΦ". iModIntro. iFrame.
+  iPureIntro.
+  done.
+Qed.
+
+Lemma wp_decodeGetArgs enc_sl enc q (key:string) :
+  {{{
+        "%Henc" ∷ ⌜has_op_encoding enc (getOp key)⌝ ∗
+        "Hsl" ∷ own_slice_small enc_sl byteT q enc
+  }}}
+    kv.decodeGetArgs (slice_val enc_sl)
+  {{{
+        RET #(str key); True
+  }}}.
+Proof.
+  iIntros (Φ) "Hpre HΦ". iNamed "Hpre".
+  wp_call.
+  cbn in Henc. subst.
+  iDestruct (own_slice_small_sz with "Hsl") as %Hsl_sz.
+  wp_apply wp_SliceSkip.
+  { simpl in Hsl_sz. word. }
+  iDestruct (slice_small_split _ 1 with "Hsl") as "[_ Hsl]".
+  { simpl. word. }
+  rewrite skipn_cons drop_0.
+  wp_apply (wp_StringFromBytes with "[$]").
+  iIntros "_".
+  wp_pures.
+  rewrite string_to_bytes_inj.
+  by iApply "HΦ".
+Qed.
+
+Notation is_state := (is_state (sm_record:=kv_record)).
+
+Definition own_KVState (s:loc) γst (ops:list OpType) (latestVnum:u64) : iProp Σ :=
+  ∃ (kvs_loc vnums_loc:loc) (vnumsM:gmap string u64) (minVnum:u64),
+  "Hkvs" ∷ s ↦[KVState :: "kvs"] #kvs_loc ∗
+  "Hvnums" ∷ s ↦[KVState :: "vnums"] #vnums_loc ∗
+  "HminVnum" ∷ s ↦[KVState :: "minVnum"] #minVnum ∗
+  "Hkvs_map" ∷ own_map kvs_loc 1 (compute_state ops) ∗
+  "Hvnums_map" ∷ own_map vnums_loc 1 vnumsM ∗
+  "#Hst" ∷ □ (∀ (k:string),
+              (∀ (vnum':u64), ⌜int.nat vnum' <= int.nat latestVnum⌝ →
+                             ⌜int.nat (default minVnum (vnumsM !! k)) <= int.nat vnum'⌝ →
+              ∃ someOps, is_state γst vnum' someOps ∗
+                      ⌜compute_reply someOps (getOp k) = compute_reply ops (getOp k)⌝)) ∗
+  "%Hle" ∷ ⌜∀ (k:string), int.nat (default minVnum (vnumsM !! k)) <= int.nat latestVnum⌝
+.
+
+Implicit Type own_VersionedStateMachine : gname → (list OpType) → u64 → iProp Σ.
+
+Lemma wp_KVState__apply s :
+  {{{
+        True
+  }}}
+    KVState__apply #s
+  {{{
+        applyFn, RET applyFn;
+        ⌜val_ty applyFn (slice.T byteT -> (arrowT uint64T (slice.T byteT)))⌝ ∗
+        is_Versioned_applyVolatileFn applyFn (own_KVState s)
+  }}}
+.
+Proof.
+  iIntros (Φ) "_ HΦ".
+  wp_lam.
+  wp_pures.
+  iModIntro.
+  iApply "HΦ".
+  clear Φ.
+  iSplit.
+  {
+    iPureIntro. econstructor.
+  }
+  iIntros (??????? Φ) "!# Hpre HΦ".
+  iDestruct "Hpre" as "(%Henc & %Hvnum & #Hsl & Hown & #Hintermediate)".
+  iNamed "Hown".
+  wp_pures.
+  iMod (readonly_load with "Hsl") as (?) "Hsl2".
+  destruct op.
+  { (* case: put op *)
+    rewrite -Henc.
+    wp_apply (wp_SliceGet with "[$Hsl2]").
+    { done. }
+    iIntros "Hsl2".
+    wp_pures.
+    wp_apply (wp_decodePutArgs with "[$Hsl2 //]").
+    iIntros (?). iNamed 1.
+    wp_pures.
+    wp_loadField.
+    wp_loadField.
+    wp_apply (wp_MapInsert with "[$]").
+    { done. }
+    iIntros "Hvnums_map".
+
+    wp_pures.
+    wp_call.
+    wp_loadField.
+    wp_loadField.
+    wp_loadField.
+    wp_apply (wp_MapInsert_to_val with "[$Hkvs_map]").
+    iIntros "Hkvs_map".
+    wp_pures.
+
+    wp_apply wp_NewSlice.
+    iIntros (?) "Hnil".
+
+    iApply "HΦ".
+    iSplitL "Hkvs Hkvs_map Hvnums HminVnum Hvnums_map".
+    {
+      repeat iExists _; iFrame.
+      unfold compute_state.
+      rewrite foldl_snoc.
+      iFrame.
+      iSplitL.
+      {
+        iModIntro.
+        iIntros.
+        rewrite /typed_map.map_insert /= in H0.
+        destruct (decide (k = s0)).
+        { subst. rewrite lookup_insert /= in H0.
+          replace (vnum) with (vnum') by word.
+          iExists _. by iDestruct "Hintermediate" as "[_ $]".
+        }
+        assert (compute_reply (ops ++ [putOp s0 s1]) (getOp k) =
+                  compute_reply (ops) (getOp k)) as Heq; last setoid_rewrite Heq.
+        {
+          rewrite /compute_reply /compute_state.
+          rewrite foldl_snoc /=.
+          by rewrite lookup_insert_ne.
+        }
+        rewrite lookup_insert_ne in H0; last done.
+        destruct (decide (int.nat vnum' <= int.nat latestVnum)).
+        { by iApply "Hst". }
+        destruct (decide (int.nat vnum' = int.nat vnum)).
+        { replace (vnum') with (vnum) by word.
+          iExists _.
+          iDestruct "Hintermediate" as "[_ $]".
+          iPureIntro.
+          by rewrite /compute_reply /compute_state foldl_snoc /= lookup_insert_ne.
+        }
+        {
+          iDestruct "Hintermediate" as "[Hint _]".
+          iSpecialize ("Hint" $! vnum' with "[%] [%]").
+          { word. }
+          { word. }
+          iExists _. by iFrame "Hint".
+        }
+      }
+      {
+        iPureIntro. intros.
+        destruct (decide (k = s0)).
+        { subst.
+          by rewrite /typed_map.map_insert lookup_insert /=.
+        }
+        {
+          rewrite /typed_map.map_insert lookup_insert_ne /=; last done.
+          transitivity (int.nat latestVnum).
+          { apply Hle. }
+          word.
+        }
+      }
+    }
+    simpl.
+    rewrite replicate_0.
+    iDestruct (own_slice_to_small with "Hnil") as "$".
+  }
+  { (* case: get op *)
+    wp_pures.
+    rewrite -Henc.
+    wp_apply (wp_SliceGet with "[$Hsl2]").
+    { done. }
+    iIntros "Hsl2".
+    wp_pures.
+    wp_apply (wp_SliceGet with "[$Hsl2]").
+    { done. }
+    iIntros "Hsl2".
+    wp_pures.
+    wp_apply (wp_decodeGetArgs with "[$Hsl2 //]").
+
+    wp_loadField.
+    wp_apply (wp_MapInsert with "[$]").
+    { done. }
+    iIntros "Hvnums_map".
+    wp_pures.
+
+    (* TODO: separate lemma *)
+    wp_call.
+    wp_loadField.
+    wp_apply (wp_MapGet with "[$Hkvs_map]").
+    iIntros (??) "[%Hlookup Hkvs_map]".
+    wp_pures.
+    wp_apply wp_StringToBytes.
+    iIntros (?) "Hrep_sl".
+
+    iApply "HΦ".
+    iSplitL "Hkvs Hkvs_map Hvnums HminVnum Hvnums_map".
+    {
+      repeat iExists _; iFrame.
+      unfold compute_state.
+      rewrite foldl_snoc.
+      iFrame.
+      iSplitL.
+      2: {
+        iPureIntro. intros.
+        destruct (decide (k = s0)).
+        { subst.
+          by rewrite /typed_map.map_insert lookup_insert /=. }
+        { rewrite /typed_map.map_insert lookup_insert_ne /=; last done.
+          transitivity (int.nat latestVnum).
+          { apply Hle. }
+          word. }
+      }
+      iModIntro.
+      iIntros.
+      rewrite /typed_map.map_insert /= in H0.
+      destruct (decide (k = s0)).
+      { subst. rewrite lookup_insert /= in H0.
+        replace (vnum) with (vnum') by word.
+        iExists _. by iDestruct "Hintermediate" as "[_ $]".
+      }
+      eassert (compute_reply (ops ++ [_]) (getOp k) =
+                compute_reply (ops) (getOp k)) as Heq; last setoid_rewrite Heq.
+      {
+        rewrite /compute_reply /compute_state.
+        rewrite foldl_snoc /=. done.
+      }
+      rewrite lookup_insert_ne in H0; last done.
+      destruct (decide (int.nat vnum' <= int.nat latestVnum)).
+      { by iApply "Hst". }
+      destruct (decide (int.nat vnum' = int.nat vnum)).
+      { replace (vnum') with (vnum) by word.
+        iExists _.
+        iDestruct "Hintermediate" as "[_ $]".
+        iPureIntro.
+        by rewrite /compute_reply /compute_state foldl_snoc /=.
+      }
+      {
+        iDestruct "Hintermediate" as "[Hint _]".
+        iSpecialize ("Hint" $! vnum' with "[%] [%]").
+        { word. }
+        { word. }
+        iExists _. by iFrame "Hint".
+      }
+    }
+    injection Hlookup as <- <-.
+    iDestruct (own_slice_to_small with "Hrep_sl") as "$".
+  }
+Qed.
+
+Lemma wp_KVState__applyReadonly s :
+  {{{
+        True
+  }}}
+    KVState__applyReadonly #s
+  {{{
+        applyReadonlyFn, RET applyReadonlyFn;
+        ⌜val_ty applyReadonlyFn (slice.T byteT -> (prodT uint64T (slice.T byteT)))⌝ ∗
+        is_Versioned_applyReadonlyFn applyReadonlyFn (own_KVState s)
+  }}}
+.
+Proof.
+  iIntros (Φ) "_ HΦ".
+  wp_call.
+  iModIntro.
+  iApply "HΦ".
+  clear Φ.
+  iSplit.
+  {
+    iPureIntro. econstructor.
+  }
+  iIntros (?????? Φ) "!# Hpre HΦ".
+  iDestruct "Hpre" as "(%Hro & %Henc & #Hsl & Hown)".
+  wp_pures.
+  destruct op.
+  { by exfalso. }
+  rewrite /kv_record /= in Henc.
+  rewrite <- Henc.
+  iMod (readonly_load with "Hsl") as (?) "Hsl2".
+  wp_apply (wp_SliceGet with "[$Hsl2]").
+  { done. }
+  iIntros "Hsl2".
+  wp_pures.
+  wp_apply (wp_decodeGetArgs with "[$Hsl2 //]").
+  iNamed "Hown".
+  wp_pures.
+  wp_call.
+  wp_loadField.
+  wp_apply (wp_MapGet with "Hkvs_map").
+  iIntros (??) "[%Hkv_lookup Hkvs_map]".
+  wp_pures.
+  wp_apply wp_StringToBytes.
+  iIntros (?) "Hrep_sl".
+  wp_loadField.
+  wp_apply (wp_MapGet with "Hvnums_map").
+  iIntros (??) "(%Hlookup & Hvnums_map)".
+  wp_pures.
+  wp_if_destruct.
+  {
+    wp_pures. iApply "HΦ". iModIntro.
+    apply map_get_true in Hlookup.
+    pose proof (Hle s0) as Hle2.
+    rewrite Hlookup /= in Hle2.
+    iSplitR. { iPureIntro. word. }
+    injection Hkv_lookup as <- ?.
+    iDestruct (own_slice_to_small with "Hrep_sl") as "$".
+    rewrite /kv_record /compute_reply /compute_state /=.
+    iSplitL.
+    { repeat iExists _; iFrame "∗#%". }
+    iSpecialize ("Hst" $! s0).
+    rewrite Hlookup /=.
+    iModIntro. iIntros.
+    iApply "Hst".
+    { iPureIntro. word. }
+    { iPureIntro. word. }
+  }
+  {
+    wp_loadField. wp_pures. iApply "HΦ". iModIntro.
+    apply map_get_false in Hlookup as [Hlookup Hv].
+    subst.
+    pose proof (Hle s0) as Hle2.
+    rewrite Hlookup /= in Hle2.
+    iSplitR. { iPureIntro. word. }
+    injection Hkv_lookup as <- ?.
+    iDestruct (own_slice_to_small with "Hrep_sl") as "$".
+    rewrite /kv_record /compute_reply /compute_state /=.
+    iSplitL.
+    { repeat iExists _; iFrame "∗#%". }
+    iSpecialize ("Hst" $! s0).
+    rewrite Hlookup /=.
+    iModIntro. iIntros.
+    iApply "Hst".
+    { iPureIntro. word. }
+    { iPureIntro. word. }
+  }
+Qed.
+
+Lemma wp_KVState__setState s :
+  {{{
+        True
+  }}}
+    KVState__setState #s
+  {{{
+        setFn, RET setFn;
+        ⌜val_ty setFn ((slice.T byteT) -> (arrowT uint64T unitT))%ht⌝ ∗
+        is_Versioned_setStateFn setFn (own_KVState s)
+  }}}
+.
+Proof.
+  iIntros (Φ) "_ HΦ".
+  wp_call.
+  iModIntro.
+  iApply "HΦ".
+  clear Φ.
+  iSplit.
+  {
+    iPureIntro. econstructor.
+  }
+
+  iIntros (???????? Φ) "!# Hpre HΦ".
+  iDestruct "Hpre" as "(%Hsnap & #Hsnap_sl & Hown & #HstNew)".
+  wp_pures.
+
+  iNamed "Hown".
+  iMod (readonly_load with "Hsnap_sl") as (?) "Hsnap_sl2".
+  wp_storeField.
+  wp_apply (wp_NewMap string).
+  iClear "Hvnums_map".
+  iIntros (?) "Hvnums_map".
+  wp_storeField.
+  wp_apply (wp_DecodeStringMap with "[Hsnap_sl2]").
+  {
+    rewrite /kv_record.(Sm.has_snap_encoding) /= in Hsnap.
+    iSplitR; first done.
+    iApply to_named.
+    iExactEq "Hsnap_sl2".
+    f_equal.
+    instantiate (1:=[]).
+    rewrite app_nil_r.
+    done.
+  }
+  iIntros (mptr) "Hmap".
+  wp_storeField.
+  iApply "HΦ".
+  iModIntro. repeat iExists _; iFrame.
+  iSplitR.
+  { iModIntro. iIntros.
+    assert (int.nat vnum' = int.nat vnum).
+    { rewrite lookup_empty /= in H0. word. }
+    replace (vnum) with vnum' by word.
+    by iExists _; iFrame "HstNew". }
+  iPureIntro. intros. rewrite lookup_empty /=. word.
+Qed.
+
+Lemma wp_KVState__getState (s:loc) :
+  ⊢ is_Versioned_getStateFn (λ: <>, KVState__getState #s) (own_KVState s).
+Proof.
+  iIntros (??? Φ) "!# Hpre HΦ".
+  iDestruct "Hpre" as "Hown".
+  wp_pures.
+  wp_call.
+  iNamed "Hown".
+  wp_loadField.
+  iApply wp_fupd.
+  wp_apply (wp_EncodeStringMap with "Hkvs_map").
+  iIntros (??) "(Hmap & Henc & %Henc)".
+  iDestruct (own_slice_to_small with "Henc") as "Henc_sl".
+  iMod (readonly_alloc_1 with "Henc_sl") as "#Henc_sl".
+  iApply "HΦ".
+  iModIntro.
+  iFrame "#".
+  iSplitL; last done.
+  repeat iExists _; iFrame "∗#%".
+Qed.
+
+Notation is_InMemoryStateMachine := (is_InMemoryStateMachine (sm_record:=kv_record)).
+
+Lemma wp_makeVersionedStateMachine :
+  {{{
+        True
+  }}}
+    makeVersionedStateMachine #()
+  {{{
+      sm own_MemStateMachine, RET #sm;
+        is_VersionedStateMachine sm own_MemStateMachine ∗
+        (∀ γst, is_state γst (U64 0) [] -∗ own_MemStateMachine γst [] (U64 0))
+  }}}.
+Proof.
+  iIntros (Φ) "Hpre HΦ".
+  wp_call.
+
+  wp_apply (wp_allocStruct).
+  { Transparent slice.T. repeat econstructor. Opaque slice.T. }
+  iIntros (s) "Hs".
+  iDestruct (struct_fields_split with "Hs") as "Hs".
+  iNamed "Hs".
+  wp_pures.
+  wp_apply (wp_NewMap string).
+  iIntros (?) "Hmap".
+  wp_storeField.
+  wp_apply (wp_NewMap string).
+  iIntros (?) "Hvnums_map".
+  wp_storeField.
+  wp_apply (wp_KVState__apply).
+  iIntros (?) "[% #His_apply]".
+  wp_apply (wp_KVState__applyReadonly).
+  iIntros (?) "[% #His_applyReadonly]".
+  wp_apply (wp_KVState__setState).
+  iIntros (?) "[% #His_setstate]".
+  iApply wp_fupd.
+  wp_apply (wp_allocStruct).
+  {
+    repeat econstructor; try done.
+  }
+  iIntros (?) "Hl".
+  iDestruct (struct_fields_split with "Hl") as "HH".
+  iNamed "HH".
+  iMod (readonly_alloc_1 with "ApplyVolatile") as "#Happly".
+  iMod (readonly_alloc_1 with "ApplyReadonly") as "#HapplyReadonly".
+  iMod (readonly_alloc_1 with "GetState") as "#Hgetstate".
+  iMod (readonly_alloc_1 with "SetState") as "#HsetState".
+  iApply "HΦ".
+  iSplitR.
+  {
+    repeat iExists _. iModIntro.
+    iFrame "#". iApply wp_KVState__getState.
+  }
+  iModIntro.
+  iIntros (?) "#?".
+  repeat iExists _; iFrame.
+  iSplitL.
+  { iModIntro. iIntros. rewrite lookup_empty /= in H3.
+    replace (int.nat (U64 0)) with (0) in * by word.
+    assert (int.nat vnum' = int.nat 0) by word.
+    replace (vnum') with (U64 0) by word.
+    iExists _; by iFrame "#".
+  }
+  iPureIntro. intros. rewrite lookup_empty /= //.
+Qed.
+
+End local_proof.
